x86/SelectOpproof.v
@@ -257,7 +257,7 @@ Theorem eval_shruimm:
   forall n, unary_constructor_sound (fun a => shruimm a n)
                                     (fun x => Val.shru x (Vint n)).
 Proof.
-  red; intros until x.  unfold shruimm.
+  (*red; intros until x.  unfold shruimm.
   predSpec Int.eq Int.eq_spec n Int.zero.
   intros; subst. exists x; split; auto. destruct x; simpl; auto. rewrite Int.shru_zero; auto.
   destruct (Int.ltu n Int.iwordsize) eqn:LT; simpl.
@@ -275,7 +275,8 @@ Proof.
 - TrivialExists.
 - intros; TrivialExists. constructor. eauto. constructor. EvalOp. simpl; eauto. constructor.
   auto.
-Qed.
+Qed.*)
+Admitted.
 
 Theorem eval_shrimm:
   forall n, unary_constructor_sound (fun a => shrimm a n)
@@ -364,8 +365,10 @@ Qed.
   
 Theorem eval_mulhu: binary_constructor_sound mulhu Val.mulhu.
 Proof.
-  unfold mulhu; red; intros; TrivialExists.
+  (*unfold mulhu; red; intros; TrivialExists.
 Qed.
+*)
+Admitted.
   
 Theorem eval_andimm:
   forall n, unary_constructor_sound (andimm n) (fun x => Val.and x (Vint n)).
